update

chapter2/E2_2.thy
@@ -4,7 +4,7 @@ begin
 
 datatype nat = nil | suc nat
 
-fun add :: "nat ⇒ nat ⇒ nat" where
+fun add :: "nat \<Rightarrow> nat \<Rightarrow> nat" where
   "add nil n = n" |
   "add (suc m) n = suc (add m n)"
 
@@ -28,7 +28,7 @@ lemma add_commut : "add m n = add n m"
   apply(auto)
   done
 
-fun double :: "nat⇒ nat" where
+fun double :: "nat\<Rightarrow> nat" where
   "double nil = nil" |
   "double (suc m) = suc (suc (double m))"
 
