chapter2/E2_3.thy
@@ -2,13 +2,13 @@ theory E2_3
   imports Main
 begin
 
-fun count :: "'a ⇒ 'a list ⇒ nat" where
+fun count :: "'a \<Rightarrow> 'a list \<Rightarrow> nat" where
   "count x [] = 0" |
   "count x (y # xs) = If (x = y) (Suc (count x xs)) (count x xs)"
 
 value "count (1::nat) [1, 2, 3, 1, 3, 1]"
 
-lemma count_lt : "count x xs ≤ length xs"
+lemma count_lt : "count x xs \<le> length xs"
   apply(induction xs)
   apply(auto)
   done
