chapter3/E3_1.thy
@@ -4,30 +4,29 @@ begin
 
 datatype 'a tree = Tip | Node "'a tree" 'a "'a tree"
 
-fun set :: "'a tree ⇒ 'a set" where
+fun set :: "'a tree \<Rightarrow> 'a set" where
   "set Tip = {}" |
-  "set (Node l v r) = (set l) ∪ {v} ∪ (set r)"
+  "set (Node l v r) = (set l) \<union> {v} \<union> (set r)"
 
-fun ord :: "int tree ⇒ bool" where
+fun ord :: "int tree \<Rightarrow> bool" where
   "ord Tip = True" |
   "ord (Node Tip v Tip) = True" |
-  "ord (Node (Node ll lv lr) v Tip) = ((lv < v) ∧ (ord (Node ll lv lr)))" |
-  "ord (Node Tip v (Node rl rv rr)) = ((v < rv) ∧ (ord (Node rl rv rr)))" |
-  "ord (Node (Node ll lv lr) v (Node rl rv rr)) = ((lv < v) ∧ (v < rv) ∧ (ord (Node ll lv lr)) ∧ (ord (Node rl rv rr)))"
+  "ord (Node (Node ll lv lr) v Tip) = ((lv < v) \<and> (ord (Node ll lv lr)))" |
+  "ord (Node Tip v (Node rl rv rr)) = ((v < rv) \<and> (ord (Node rl rv rr)))" |
+  "ord (Node (Node ll lv lr) v (Node rl rv rr)) = ((lv < v) \<and> (v < rv) \<and> (ord (Node ll lv lr)) \<and> (ord (Node rl rv rr)))"
 
-fun ins :: "int tree ⇒ int ⇒ int tree" where
+fun ins :: "int tree \<Rightarrow> int \<Rightarrow> int tree" where
   "ins Tip x = Node Tip x Tip" |
   "ins (Node l v r) x = (if x = v then (Node l v r) else (if v < x then (Node l v (ins r x)) else (Node (ins l x) v r)))"
 
-lemma "set (ins t x) = {x} ∪ set t"
+lemma "set (ins t x) = {x} \<union> set t"
   apply(induction t)
   apply(auto)
   done
 
-lemma "ord t ⟹ ord (ins t i)"
+lemma "ord t \<Longrightarrow> ord (ins t i)"
   apply(induction t rule: ord.induct)
   apply(auto)
   done
 
 end
-
