chapter3/E3_4.thy
@@ -2,30 +2,30 @@ theory E3_4
   imports Main
 begin
 
-inductive star :: "('a ⇒ 'a ⇒ bool) ⇒ 'a ⇒ 'a ⇒ bool" for r where
+inductive star :: "('a \<Rightarrow> 'a \<Rightarrow> bool) \<Rightarrow> 'a \<Rightarrow> 'a \<Rightarrow> bool" for r where
 refl : "star r x x" |
-step : "r x y ⟹ star r y z ⟹ star r x z"
+step : "r x y \<Longrightarrow> star r y z \<Longrightarrow> star r x z"
 
-lemma star1 [simp, intro] : "star r x y ⟹ star r y z ⟹ star r x z"
+lemma star1 [simp, intro] : "star r x y \<Longrightarrow> star r y z \<Longrightarrow> star r x z"
   apply (induction rule : star.induct)
   apply (assumption)
   by (metis step)
 
-lemma star2 [simp, intro] : "r y z ⟹ star r y z"
+lemma star2 [simp, intro] : "r y z \<Longrightarrow> star r y z"
   by (meson star.simps)
 
-lemma star3 [simp, intro] : "star r x y ⟹ r y z ⟹ star r x z"
+lemma star3 [simp, intro] : "star r x y \<Longrightarrow> r y z \<Longrightarrow> star r x z"
   apply (induction rule : star.induct)
   apply (meson star.simps)
   by auto
 
-inductive iter :: "('a ⇒ 'a ⇒ bool) ⇒ nat ⇒ 'a ⇒ 'a ⇒ bool" for r where
+inductive iter :: "('a \<Rightarrow> 'a \<Rightarrow> bool) \<Rightarrow> nat \<Rightarrow> 'a \<Rightarrow> 'a \<Rightarrow> bool" for r where
 iter0 : "iter r n x x" |
-iter1 : "r x y ⟹ iter r 1 x y ⟹ iter r n y z ⟹ iter r (n + 1) x z" |
-iter2 : "iter r n x y ⟹ r y z ⟹ iter r (n + 1) x z" |
-iter3 : "iter r n x y ⟹ iter r m y z ⟹ iter r (m + n) x z"
+iter1 : "r x y \<Longrightarrow> iter r 1 x y \<Longrightarrow> iter r n y z \<Longrightarrow> iter r (n + 1) x z" |
+iter2 : "iter r n x y \<Longrightarrow> r y z \<Longrightarrow> iter r (n + 1) x z" |
+iter3 : "iter r n x y \<Longrightarrow> iter r m y z \<Longrightarrow> iter r (m + n) x z"
 
-lemma "star r x y ⟹ ∃ n. iter r n x y"
+lemma "star r x y \<Longrightarrow> \<exists> n. iter r n x y"
   apply (induction rule : star.induct)
   apply (simp add : iter0)
   by (metis test.iter.simps)
