chapter4/E4_5.thy
@@ -2,18 +2,18 @@ theory E4_5
   imports Main
 begin
 
-inductive star :: "('a ⇒ 'a ⇒ bool) ⇒ 'a ⇒ 'a ⇒ bool" for r where
+inductive star :: "('a \<Rightarrow> 'a \<Rightarrow> bool) \<Rightarrow> 'a \<Rightarrow> 'a \<Rightarrow> bool" for r where
 refl : "star r x x" |
-step : "r x y ⟹ star r y z ⟹ star r x z"
+step : "r x y \<Longrightarrow> star r y z \<Longrightarrow> star r x z"
 
-inductive iter :: "('a ⇒ 'a ⇒ bool) ⇒ nat ⇒ 'a ⇒ 'a ⇒ bool" for r where
+inductive iter :: "('a \<Rightarrow> 'a \<Rightarrow> bool) \<Rightarrow> nat \<Rightarrow> 'a \<Rightarrow> 'a \<Rightarrow> bool" for r where
 iter0 : "iter r n x x" |
-iter1 : "r x y ⟹ iter r 1 x y ⟹ iter r n y z ⟹ iter r (n + 1) x z" |
-iter2 : "iter r n x y ⟹ r y z ⟹ iter r (n + 1) x z" |
-iter3 : "iter r n x y ⟹ iter r m y z ⟹ iter r (m + n) x z"
+iter1 : "r x y \<Longrightarrow> iter r 1 x y \<Longrightarrow> iter r n y z \<Longrightarrow> iter r (n + 1) x z" |
+iter2 : "iter r n x y \<Longrightarrow> r y z \<Longrightarrow> iter r (n + 1) x z" |
+iter3 : "iter r n x y \<Longrightarrow> iter r m y z \<Longrightarrow> iter r (m + n) x z"
 
-lemma star_trans[simp, intro] : "star r x y ⟹ star r y z ⟹ star r x z"
-proof (induction rule : star.induct)  
+lemma star_trans[simp, intro] : "star r x y \<Longrightarrow> star r y z \<Longrightarrow> star r x z"
+proof (induction rule : star.induct)
   case (refl x)
   thus ?case by auto
 next
@@ -21,7 +21,7 @@ next
   thus ?case by (meson star.step)
 qed
 
-lemma "iter r n x y ⟹ star r x y"
+lemma "iter r n x y \<Longrightarrow> star r x y"
 proof (induction rule : iter.induct)
   case (iter0 n x)
   then show ?case by (meson star.simps)
