chapter4/E4_6.thy
@@ -2,23 +2,23 @@ theory E4_6
   imports Main
 begin
 
-fun elems :: "'a list ⇒ 'a set" where
+fun elems :: "'a list \<Rightarrow> 'a set" where
   "elems [] = {}" |
-  "elems (x # xs) = {x} ∪ elems xs"
+  "elems (x # xs) = {x} \<union> elems xs"
 
-lemma "x ∈ elems xs ⟹ ∃ ys zs. xs = ys @ x # zs ∧ x ∉ elems ys"
+lemma "x \<in> elems xs \<Longrightarrow> \<exists> ys zs. xs = ys @ x # zs \<and> x \<notin> elems ys"
 proof (induction xs)
 case Nil
   then show ?case by auto
 next
   case (Cons a xs)
-  then show ?case 
+  then show ?case
   proof (cases "x = a")
     case True
     then show ?thesis by fastforce
   next
     case False
-    hence "x ∈ elems xs" using Cons.prems by auto 
+    hence "x \<in> elems xs" using Cons.prems by auto
     thus ?thesis by (metis Cons.IH False UnE append_Cons elems.simps(2) empty_iff insert_iff)
   qed
 qed
