chapter2/E2_6.thy
@@ -4,11 +4,11 @@ begin
 
 datatype 'a tree = Tip | Node "'a tree" 'a "'a tree"
 
-fun contents :: "'a tree ⇒ 'a list" where
+fun contents :: "'a tree \<Rightarrow> 'a list" where
   "contents Tip = []" |
   "contents (Node l v r) = v # ((contents l) @ (contents r))"
 
-fun sum_tree :: "nat tree ⇒ nat" where
+fun sum_tree :: "nat tree \<Rightarrow> nat" where
   "sum_tree Tip = 0" |
   "sum_tree (Node l v r) = v + (sum_tree l) + (sum_tree r)"
 
