chapter2/E2_7.thy
@@ -4,15 +4,15 @@ begin
 
 datatype 'a tree = Leaf 'a | Node "'a tree" 'a "'a tree"
 
-fun mirror :: "'a tree ⇒ 'a tree" where
+fun mirror :: "'a tree \<Rightarrow> 'a tree" where
   "mirror (Leaf v) = Leaf v" |
   "mirror (Node l v r) = Node (mirror r) v (mirror l)"
 
-fun pre_order :: "'a tree ⇒ 'a list" where
+fun pre_order :: "'a tree \<Rightarrow> 'a list" where
   "pre_order (Leaf v) = [v]" |
   "pre_order (Node l v r) = v # (pre_order l) @ (pre_order r)"
 
-fun post_order :: "'a tree ⇒ 'a list" where
+fun post_order :: "'a tree \<Rightarrow> 'a list" where
   "post_order (Leaf v) = [v]" |
   "post_order (Node l v r) = (post_order l) @ (post_order r) @ [v]"
 
@@ -27,15 +27,15 @@ lemma "pre_order (mirror t) = rev (post_order t)"
 (*
 datatype 'a tree = Til | Node "'a tree" 'a "'a tree"
 
-fun mirror :: "'a tree ⇒ 'a tree" where
+fun mirror :: "'a tree \<Rightarrow> 'a tree" where
   "mirror Til = Til" |
   "mirror (Node l v r) = Node (mirror r) v (mirror l)"
 
-fun pre_order :: "'a tree ⇒ 'a list" where
+fun pre_order :: "'a tree \<Rightarrow> 'a list" where
   "pre_order Til = []" |
   "pre_order (Node l v r) = v # (pre_order l) @ (pre_order r)"
 
-fun post_order :: "'a tree ⇒ 'a list" where
+fun post_order :: "'a tree \<Rightarrow> 'a list" where
   "post_order Til = []" |
   "post_order (Node l v r) = (post_order l) @ (post_order r) @ [v]"
 
