chapter2/E2_8.thy
@@ -2,7 +2,7 @@ theory E2_8
   imports Main
 begin
 
-fun intersperse :: "'a ⇒ 'a list ⇒ 'a list" where
+fun intersperse :: "'a \<Rightarrow> 'a list \<Rightarrow> 'a list" where
   "intersperse a [] = []" |
   "intersperse a [x] = [x]" |
   "intersperse a (x # xs) = (x # [a]) @ (intersperse a xs)"
