chapter3/E3_5.thy
@@ -4,16 +4,16 @@ begin
 
 datatype alpha = a | b
 
-inductive S :: "alpha list ⇒ bool" where
+inductive S :: "alpha list \<Rightarrow> bool" where
 S0 : "S []" |
-S1 : "S w ⟹ S (a # w @ [b])" |
-S2 : "S w ⟹ S v ⟹ S (w @ v)"
+S1 : "S w \<Longrightarrow> S (a # w @ [b])" |
+S2 : "S w \<Longrightarrow> S v \<Longrightarrow> S (w @ v)"
 
-inductive T :: "alpha list ⇒ bool" where
+inductive T :: "alpha list \<Rightarrow> bool" where
 T0 : "T []" |
-T1 : "T w ⟹ T v ⟹ T (w @ [a] @ v @ [b])"
+T1 : "T w \<Longrightarrow> T v \<Longrightarrow> T (w @ [a] @ v @ [b])"
 
-lemma T_cat [simp] : "T v ⟹ T w ⟹ T (w @ v)"
+lemma T_cat [simp] : "T v \<Longrightarrow> T w \<Longrightarrow> T (w @ v)"
   apply (induction rule : T.induct)
   apply simp
   by (metis T.simps append.assoc)
