chapter4/E4_1.thy
@@ -2,9 +2,9 @@ theory E4_1
   imports Main
 begin
 
-lemma assumes T: "∀ x y. T x y ∨ T y x"
-  and A: "∀ x y. A x y ∧ A y x ⟶ x = y"
-  and TA: "∀ x y. T x y ⟶ A x y" and "A x y"
+lemma assumes T: "\<forall> x y. T x y \<or> T y x"
+  and A: "\<forall> x y. A x y \<and> A y x \<longrightarrow> x = y"
+  and TA: "\<forall> x y. T x y \<longrightarrow> A x y" and "A x y"
   shows "T x y"
 proof -
   from T A TA `A x y` show "T x y" by blast
