chapter4/E4_2.thy
@@ -2,18 +2,18 @@ theory E4_2
   imports Main
 begin
 
-lemma "∃ ys zs. xs = ys @ zs ∧ (length ys = length zs ∨ length ys = length zs + 1)"
+lemma "\<exists> ys zs. xs = ys @ zs \<and> (length ys = length zs \<or> length ys = length zs + 1)"
 proof cases
   let ?l1 = "take ((length xs div 2)) xs"
   let ?l2 = "drop ((length xs div 2)) xs"
   assume "even (length xs)"
-  hence "xs = ?l1 @ ?l2 ∧ length ?l1 = length ?l2" by auto
+  hence "xs = ?l1 @ ?l2 \<and> length ?l1 = length ?l2" by auto
   thus ?thesis by blast
 next
   let ?l1 = "take ((length xs div 2) + 1) xs"
   let ?l2 = "drop ((length xs div 2) + 1) xs"
   assume "odd (length xs)"
-  hence "xs = ?l1 @ ?l2 ∧ length ?l1 = length ?l2 + 1" by (smt add.commute add_diff_cancel_right' append_take_drop_id left_add_twice length_append length_drop odd_two_times_div_two_succ)
+  hence "xs = ?l1 @ ?l2 \<and> length ?l1 = length ?l2 + 1" by (smt add.commute add_diff_cancel_right' append_take_drop_id left_add_twice length_append length_drop odd_two_times_div_two_succ)
   thus ?thesis by blast
 qed
 
