chapter4/E4_7.thy
@@ -1,15 +1,15 @@
-theory test
+theory E4_7
   imports Main
 begin
 
 datatype alpha = a | b
 
-inductive S :: "alpha list ⇒ bool" where
+inductive S :: "alpha list \<Rightarrow> bool" where
 S0 : "S []" |
-S1 : "S w ⟹ S (a # w @ [b])" |
-S2 : "S w ⟹ S v ⟹ S (w @ v)"
+S1 : "S w \<Longrightarrow> S (a # w @ [b])" |
+S2 : "S w \<Longrightarrow> S v \<Longrightarrow> S (w @ v)"
 
-fun balanced :: "nat ⇒ alpha list ⇒ bool" where
+fun balanced :: "nat \<Rightarrow> alpha list \<Rightarrow> bool" where
   "balanced 0 [] = True" |
   "balanced n (a # w) = balanced (n + 1) w" |
   "balanced n (b # w) = balanced (n - 1) w" |
